src/Init/Data/FloatArray/Basic.lean
@@ -55,17 +55,17 @@ def get? (ds : FloatArray) (i : Nat) : Option Float :=
   else
     none
 
-instance : GetElem FloatArray Nat Float fun xs i => i < xs.size where
+instance : GetElemBase FloatArray Nat Float fun xs i => i < xs.size where
   getElem xs i h := xs.get ⟨i, h⟩
-  getElem? xs i := if h : i < xs.size then some (xs.get ⟨i, h⟩) else none
-  getElem! xs i := if h : i < xs.size then xs.get ⟨i, h⟩ else outOfBounds
+
+instance : GetElem FloatArray Nat Float fun xs i => i < xs.size where
 
 instance : LawfulGetElem FloatArray Nat Float fun xs i => i < xs.size where
 
-instance : GetElem FloatArray USize Float fun xs i => i.val < xs.size where
+instance : GetElemBase FloatArray USize Float fun xs i => i.val < xs.size where
   getElem xs i h := xs.uget i h
-  getElem? xs i := if h : i.val < xs.size then some (xs.uget i h) else none
-  getElem! xs i := if h : i.val < xs.size then xs.uget i h else outOfBounds
+
+instance : GetElem FloatArray USize Float fun xs i => i.val < xs.size where
 
 instance : LawfulGetElem FloatArray USize Float fun xs i => i.val < xs.size where
 
