src/Lean/Data/PersistentHashMap.lean
@@ -158,10 +158,10 @@ partial def findAux [BEq α] : Node α β → USize → α → Option β
 def find? {_ : BEq α} {_ : Hashable α} : PersistentHashMap α β → α → Option β
   | { root }, k => findAux root (hash k |>.toUSize) k
 
-instance {_ : BEq α} {_ : Hashable α} : GetElem (PersistentHashMap α β) α (Option β) fun _ _ => True where
+instance {_ : BEq α} {_ : Hashable α} : GetElemBase (PersistentHashMap α β) α (Option β) fun _ _ => True where
   getElem m i _ := m.find? i
-  getElem? m i := some (m.find? i) -- Not really sure what should go here. We're meant to be returning an `Option (Option β)`.
-  getElem! m i := m.find? i
+
+instance {_ : BEq α} {_ : Hashable α} : GetElem (PersistentHashMap α β) α (Option β) fun _ _ => True where
 
 instance {_ : BEq α} {_ : Hashable α} : LawfulGetElem (PersistentHashMap α β) α (Option β) fun _ _ => True where
 
